@prefix general: <https://github.com/GAIA-X4PLC-AAD/ontology-management-base/tree/main/general/> .
@prefix manifest: <https://github.com/GAIA-X4PLC-AAD/ontology-management-base/tree/main/manifest/> .
@prefix gx: <https://registry.lab.gaia-x.eu/development/api/trusted-shape-registry/v1/shapes/jsonld/trustframework#> .
@prefix owl: <http://www.w3.org/2002/07/owl#> .
@prefix rdfs: <http://www.w3.org/2000/01/rdf-schema#> .
@prefix dcterms: <http://purl.org/dc/terms/> .
@prefix foaf: <http://xmlns.com/foaf/spec/> .
@prefix org: <http://www.w3.org/ns/org#> .
@prefix prov: <http://www.w3.org/ns/prov#> .
@prefix xsd: <http://www.w3.org/2001/XMLSchema#> .


# Ontology metadata
general: a owl:Ontology ;
    rdfs:label "Ontology definition for general"@en ;
    rdfs:comment "General ontology with common classes for defining an asset in the simulation domain."@en ;
    
    dcterms:creator "The GAIA-X 4 PLC AAD Project Team"@en ;
    dcterms:contributor [
        a foaf:Person ;
        foaf:name "Carlo van Driesten" ;
        org:memberOf <https://www.bmwgroup.com/> ;
    ] , [
        a foaf:Person ;
        foaf:name "Mirco Nierenz" ;
        org:memberOf <https://triangraphics.de/> ;
    ] , [
        a foaf:Person ;
        foaf:name "Erik Konietzko" ;
        org:memberOf <https://www.ipk.fraunhofer.de/> ;
    ] ;  

    # Permanent identifier for the ontology (not version-specific)
    dcterms:identifier <https://ontologies.envited-x.net/general> ;

    # GitHub repository where the ontology is maintained
    dcterms:source <https://github.com/GAIA-X4PLC-AAD/ontology-management-base> ;

    # Specific GitHub release used for publishing this version
    prov:wasDerivedFrom <https://github.com/GAIA-X4PLC-AAD/ontology-management-base/releases/tag/v0.0.2> ;

    # Versioning
    owl:versionIRI <https://ontologies.envited-x.net/general/v3/ontology> ;
    owl:versionInfo "v3" ;

    # Reference to SHACL validation rules
    dcterms:conformsTo <https://ontologies.envited-x.net/general/v3/shape> ;

    # Additional references to the ENVITED Ecosystem Specification (EVES) or related ontologies
    dcterms:references <https://registry.lab.gaia-x.eu/development/api/trusted-shape-registry/v1/shapes/jsonld/trustframework#> ;
    rdfs:seeAlso <https://ascs-ev.github.io/EVES/> .

# General metadata class
general:Metadata a owl:Class ;
    rdfs:label "Metadata"@en ;
    rdfs:comment "General metadata containing information such as name and description of the simulation asset."@en ;
    rdfs:subClassOf gx:DataResource .

# Core simulation asset class
general:SimulationAsset a owl:Class ;
    rdfs:label "Simulation Asset"@en ;
    rdfs:comment "A structured digital resource that includes extensible metadata and a table of contents as a linked manifest."@en ;
    rdfs:subClassOf gx:DataResource ;
    rdfs:subClassOf [ 
        a owl:Restriction ; 
        owl:onProperty general:hasMetadata ; 
        owl:someValuesFrom general:Metadata 
    ] .

manifest:Manifest a owl:Class ;
    rdfs:label "Class definition for Manifest"@en ;
    rdfs:comment "Defines the structure as list of contents of an asset (e.g. simulation asset) using a manifest.json, including content data and license as linked properties."@en .

# Object properties
general:hasMetadata a owl:ObjectProperty ;
    rdfs:domain general:SimulationAsset ;
    rdfs:range general:Metadata ;
    rdfs:comment "Links a simulation asset to its metadata, such as name and description."@en .

general:hasManifest a owl:ObjectProperty ;
    rdfs:domain general:SimulationAsset ;
    rdfs:range manifest:Manifest ;
    rdfs:comment "Each simulation asset must have an associated manifest that describes its structure and content."@en .
