@prefix envited-x: <https://github.com/GAIA-X4PLC-AAD/ontology-management-base/tree/main/envited-x/> .
@prefix manifest: <https://github.com/GAIA-X4PLC-AAD/ontology-management-base/tree/main/manifest/> .
@prefix gx: <https://registry.lab.gaia-x.eu/development/api/trusted-shape-registry/v1/shapes/jsonld/trustframework#> .
@prefix owl: <http://www.w3.org/2002/07/owl#> .
@prefix rdfs: <http://www.w3.org/2000/01/rdf-schema#> .
@prefix dcterms: <http://purl.org/dc/terms/> .
@prefix foaf: <http://xmlns.com/foaf/spec/> .
@prefix org: <http://www.w3.org/ns/org#> .
@prefix prov: <http://www.w3.org/ns/prov#> .
@prefix xsd: <http://www.w3.org/2001/XMLSchema#> .


# Ontology metadata
envited-x: a owl:Ontology ;
    rdfs:label "Ontology definition for envited-x"@en ;
    rdfs:comment "ENVITED-X Data Space ontology with common classes for defining a digital asset in the simulation domain."@en ;
    
    dcterms:creator "The GAIA-X 4 PLC AAD Project Team"@en ;
    dcterms:contributor [
        a foaf:Person ;
        foaf:name "Carlo van Driesten" ;
        org:memberOf <https://www.bmwgroup.com/> ;
    ] , [
        a foaf:Person ;
        foaf:name "Mirco Nierenz" ;
        org:memberOf <https://triangraphics.de/> ;
    ] , [
        a foaf:Person ;
        foaf:name "Erik Konietzko" ;
        org:memberOf <https://www.ipk.fraunhofer.de/> ;
    ] ;  

    # Permanent identifier for the ontology (not version-specific)
    dcterms:identifier <https://ontologies.envited-x.net/envited-x> ;

    # GitHub repository where the ontology is maintained
    dcterms:source <https://github.com/GAIA-X4PLC-AAD/ontology-management-base> ;

    # Specific GitHub release used for publishing this version
    prov:wasDerivedFrom <https://github.com/GAIA-X4PLC-AAD/ontology-management-base/releases/tag/v0.0.2> ;

    # Versioning
    owl:versionIRI <https://ontologies.envited-x.net/envited-x/v1/ontology> ;
    owl:versionInfo "v1" ;

    # Reference to SHACL validation rules
    dcterms:conformsTo <https://ontologies.envited-x.net/envited-x/v1/shape> ;

    # Additional references to the ENVITED Ecosystem Specification (EVES) or related ontologies
    dcterms:references <https://registry.lab.gaia-x.eu/development/api/trusted-shape-registry/v1/shapes/jsonld/trustframework#> ;
    rdfs:seeAlso <https://ascs-ev.github.io/EVES/> .

# envited-x DataResource class
envited-x:DataResource a owl:Class ;
    rdfs:label "Class definition for DataResource"@en ;
    rdfs:comment "ENVITED-X DataResource containing information such as name and description of the simulation asset."@en ;
    rdfs:subClassOf gx:DataResource .

# envited-x Manifest class
envited-x:Manifest a owl:Class ;
    rdfs:label "Class definition for Manifest"@en ;
    rdfs:comment "Defines the structure as list of contents of an asset (e.g. simulation asset) using a manifest.json, including content data and license as linked properties."@en ;
    rdfs:subClassOf manifest:Manifest .

# Core simulation asset class
envited-x:SimulationAsset a owl:Class ;
    rdfs:label "Class definition for SimulationAsset"@en ;
    rdfs:comment "A structured digital resource that includes extensible metadata and a table of contents as a linked manifest."@en ;
    rdfs:subClassOf gx:DataResource ;
    rdfs:subClassOf [ 
        a owl:Restriction ; 
        owl:onProperty envited-x:hasDataResource ; 
        owl:someValuesFrom envited-x:DataResource 
    ] ;
    rdfs:subClassOf [ 
        a owl:Restriction ; 
        owl:onProperty envited-x:hasManifest ;  
        owl:someValuesFrom envited-x:Manifest
    ] .

# Object properties
envited-x:hasDataResource a owl:ObjectProperty ;
    rdfs:domain envited-x:SimulationAsset ;
    rdfs:range envited-x:DataResource ;
    rdfs:comment "Links a simulation asset to its extentable gx:DataResource metadata, such as name and description; applicable only within SimulationAsset instances."@en .

envited-x:hasManifest a owl:ObjectProperty ;
    rdfs:domain envited-x:SimulationAsset ;
    rdfs:range envited-x:Manifest ;
    rdfs:comment "Links a simulation asset to the associated manifest that describes its structure and content; applicable only within SimulationAsset instances."@en .
