@prefix hdmap: <https://github.com/GAIA-X4PLC-AAD/ontology-management-base/tree/main/hdmap/> .
@prefix envited-x: <https://github.com/GAIA-X4PLC-AAD/ontology-management-base/tree/main/envited-x/> .
@prefix manifest: <https://github.com/GAIA-X4PLC-AAD/ontology-management-base/tree/main/manifest/> .
@prefix georeference: <https://github.com/GAIA-X4PLC-AAD/ontology-management-base/tree/main/georeference/> .
@prefix owl: <http://www.w3.org/2002/07/owl#> .
@prefix dcterms: <http://purl.org/dc/terms/> .
@prefix foaf: <http://xmlns.com/foaf/spec/> .
@prefix org: <http://www.w3.org/ns/org#> .
@prefix prov: <http://www.w3.org/ns/prov#> .
@prefix rdfs: <http://www.w3.org/2000/01/rdf-schema#> .
@prefix xsd: <http://www.w3.org/2001/XMLSchema#> .


hdmap: a owl:Ontology ;
    rdfs:label "Ontology definition for hdmap"@en ;
    rdfs:comment "An ontology with common classes to describe a high-definition map (HD map) assets used in simulation."@en ;
    
    dcterms:creator "The GAIA-X 4 PLC AAD Project Team"@en ;
    dcterms:contributor [
        a foaf:Person ;
        foaf:name "Carlo van Driesten" ;
        org:memberOf <https://www.bmwgroup.com/> ;
    ] , [
        a foaf:Person ;
        foaf:name "Sebastian Tuttas" ;
        org:memberOf <https://www.3d-mapping.de/> ;
    ] , [
        a foaf:Person ;
        foaf:name "Mirco Nierenz" ;
        org:memberOf <https://triangraphics.de/> ;
    ] ;  

    # Permanent identifier for the ontology (not version-specific)
    dcterms:identifier <https://ontologies.envited-x.net/hdmap> ;

    # GitHub repository where the ontology is maintained
    dcterms:source <https://github.com/GAIA-X4PLC-AAD/ontology-management-base> ;

    # Specific GitHub release used for publishing this version
    prov:wasDerivedFrom <https://github.com/GAIA-X4PLC-AAD/ontology-management-base/releases/tag/v0.0.2> ;

    # Versioning
    owl:versionIRI <https://ontologies.envited-x.net/hdmap/v3/ontology> ;
    owl:versionInfo "v3" ;

    # Reference to SHACL validation rules
    dcterms:conformsTo <https://ontologies.envited-x.net/hdmap/v3/shape> ;

    # Additional references to documentation or related ontologies
    dcterms:references <https://github.com/GAIA-X4PLC-AAD/ontology-management-base/tree/main/envited-x/> ;
    rdfs:seeAlso <https://ascs-ev.github.io/EVES/> .


#### Classes

hdmap:HdMap a owl:Class ;
    rdfs:label "Class definition for HdMap"@en ;
    rdfs:comment "General properties for defining a high-definition map (HD map) asset used in simulation environments, such as format, content, quantity and quality properties."@en ;
    rdfs:subClassOf envited-x:SimulationAsset ;
    rdfs:subClassOf [
        a owl:Restriction ;
        owl:onProperty hdmap:hasDataResourceExtension ;
        owl:someValuesFrom hdmap:DataResourceExtension
    ] ;
    rdfs:subClassOf [
        a owl:Restriction ;
        owl:onProperty hdmap:hasDataResource ;
        owl:someValuesFrom envited-x:DataResource
    ] ;
    rdfs:subClassOf [
        a owl:Restriction ;
        owl:onProperty hdmap:hasManifest ;
        owl:someValuesFrom envited-x:Manifest
    ] .

hdmap:DataResourceExtension a owl:Class ;
    rdfs:label "Class definition for DataResourceExtension"@en ;
    rdfs:comment "HD map DataResourceExtension containing additional metadata information of the simulation asset."@en ;
    rdfs:subClassOf envited-x:DataResourceExtension ;
    rdfs:subClassOf [
        a owl:Restriction ;
        owl:onProperty hdmap:hasContent ;
        owl:someValuesFrom hdmap:Content
    ] , [
        a owl:Restriction ;
        owl:onProperty hdmap:hasDataSource ;
        owl:someValuesFrom hdmap:DataSource
    ] , [
        a owl:Restriction ;
        owl:onProperty hdmap:hasFormat ;
        owl:someValuesFrom hdmap:Format
    ] , [
        a owl:Restriction ;
        owl:onProperty hdmap:hasQuality ;
        owl:someValuesFrom hdmap:Quality
    ] , [
        a owl:Restriction ;
        owl:onProperty hdmap:hasQuantity ;
        owl:someValuesFrom hdmap:Quantity
    ] , [
        a owl:Restriction ;
        owl:onProperty hdmap:hasRange2D ;
        owl:someValuesFrom hdmap:Range2D
    ] , [
        a owl:Restriction ;
        owl:onProperty hdmap:hasGeoreference ;
        owl:someValuesFrom georeference:Georeference
    ] .

hdmap:Content a owl:Class ;
    rdfs:label "Class definition for Content"@en ;
    rdfs:comment "Defines the content (road types, lane types, object types, traffic direction) of the HD map asset."@en ;
    rdfs:subClassOf envited-x:Content .

hdmap:DataSource a owl:Class ;
    rdfs:label "Class definition for DataSource"@en ;
    rdfs:comment "Defines which data resources or measurement systems were used to create the HD map asset."@en ;
    rdfs:subClassOf envited-x:DataSource .

hdmap:Format a owl:Class ;
    rdfs:label "Class definition for Format"@en ;
    rdfs:comment "Contains properties to describe the format of the HD map asset."@en ;
    rdfs:subClassOf envited-x:Format .

hdmap:Quality a owl:Class ;
    rdfs:label "Class definition for Quality"@en ;
    rdfs:comment "Contains properties to describe the accuracy of the HD map asset."@en ;
    rdfs:subClassOf envited-x:Quality .

hdmap:Quantity a owl:Class ;
    rdfs:label "Class definition for Quantity"@en ;
    rdfs:comment "Contains properties to describe the quantity (e.g. number of intersections, traffic lights, signs, length, range of speed limits/elevations) of the HD map asset."@en ;
    rdfs:subClassOf envited-x:Quanitiy .

# Used in Quanitiy
hdmap:Range2D a owl:Class ;
    rdfs:label "Class definition for Range2D"@en ;
    rdfs:comment "Range2D definition with minimum to maximum data property usable in the HD map asset."@en .

#### Object properties

### hasDataResourceExtension (HdMap -> DataResourceExtension)
hdmap:hasDataResourceExtension a owl:ObjectProperty ;
    rdfs:label "Object property: hasDataResourceExtension"@en ;
    rdfs:comment "Links an HD map asset to its specific metadata (DataResourceExtension), which may contain additional HD map-specific attributes."@en ;
    rdfs:subPropertyOf envited-x:hasDataResourceExtension ;
    rdfs:domain hdmap:HdMap ;
    rdfs:range hdmap:DataResourceExtension .

### hasDataResource (HdMap -> envited-x:DataResource)
hdmap:hasDataResource a owl:ObjectProperty ;
    rdfs:label "Object property: hasDataResource"@en ;
    rdfs:comment "Links an HD map asset to a standard DataResource instance from envited-x."@en ;
    rdfs:subPropertyOf envited-x:hasDataResource ;
    rdfs:domain hdmap:HdMap ;
    rdfs:range envited-x:DataResource .

### hasManifest (HdMap -> envited-x:Manifest)
hdmap:hasManifest a owl:ObjectProperty ;
    rdfs:label "Object property: hasManifest"@en ;
    rdfs:comment "Links an HD map asset to its specific manifest, extending the standard manifest structure from envited-x."@en ;
    rdfs:subPropertyOf envited-x:hasManifest ;
    rdfs:domain hdmap:HdMap ;
    rdfs:range envited-x:Manifest .

### hasContent (DataResourceExtension -> Content)
hdmap:hasContent a owl:ObjectProperty ;
    rdfs:label "Object property: hasContent"@en ;
    rdfs:comment "Links a DataResourceExtension to an instance of hdmap:Content that describes the HD map`s content."@en ;
    rdfs:subPropertyOf envited-x:hasContent ;
    rdfs:domain hdmap:DataResourceExtension ;
    rdfs:range hdmap:Content .

### hasDataSource (DataResourceExtension -> DataSource)
hdmap:hasDataSource a owl:ObjectProperty ;
    rdfs:label "Object property: hasDataSource"@en ;
    rdfs:comment "Links a DataResourceExtension to an instance of hdmap:DataSource that describes how the HD map was created."@en ;
rdfs:subPropertyOf envited-x:hasDataSource ;
    rdfs:domain hdmap:DataResourceExtension ;
    rdfs:range hdmap:DataSource .

### hasFormat (DataResourceExtension -> Format)
hdmap:hasFormat a owl:ObjectProperty ;
    rdfs:label "Object property: hasFormat"@en ;
    rdfs:comment "Links a DataResourceExtension to an instance of hdmap:Format that describes the HD map`s format details."@en ;
    rdfs:subPropertyOf envited-x:hasFormat ;
    rdfs:domain hdmap:DataResourceExtension ;
    rdfs:range hdmap:Format .

### hasQuality (DataResourceExtension -> Quality)
hdmap:hasQuality a owl:ObjectProperty ;
    rdfs:label "Object property: hasQuality"@en ;
    rdfs:comment "Links a DataResourceExtension to an instance of hdmap:Quality describing the HD map`s quality or accuracy aspects."@en ;
    rdfs:subPropertyOf envited-x:hasQuality ;
    rdfs:domain hdmap:DataResourceExtension ;
    rdfs:range hdmap:Quality .

### hasQuantity (DataResourceExtension -> Quantity)
hdmap:hasQuantity a owl:ObjectProperty ;
    rdfs:label "Object property: hasQuantity"@en ;
    rdfs:comment "Links a DataResourceExtension to an instance of hdmap:Quantity describing the HD map`s quantity (intersections, traffic signs, etc.)."@en ;
    rdfs:subPropertyOf envited-x:hasQuantity ;
    rdfs:domain hdmap:DataResourceExtension ;
    rdfs:range hdmap:Quantity .

### hasRange2D (DataResourceExtension -> Range2D)
hdmap:hasRange2D a owl:ObjectProperty ;
    rdfs:label "Object property: hasRange2D"@en ;
    rdfs:comment "Links a DataResourceExtension to an instance of hdmap:Range2D describing the 2D bounding area of the HD map asset."@en ;
    rdfs:domain hdmap:DataResourceExtension ;
    rdfs:range hdmap:Range2D .

### hasGeoreference (DataResourceExtension -> georeference:Georeference)
hdmap:hasGeoreference a owl:ObjectProperty ;
    rdfs:label "Object property: hasGeoreference"@en ;
    rdfs:comment "Links a DataResourceExtension to a georeference:Georeference describing how the HD map is georeferenced."@en ;
    rdfs:domain hdmap:DataResourceExtension ;
    rdfs:range georeference:Georeference .
