@prefix georeference: <https://ontologies.envited-x.net/georeference/v3/ontology> .
@prefix envited-x: <https://ontologies.envited-x.net/envited-x/v2/ontology> .
@prefix owl: <http://www.w3.org/2002/07/owl#> .
@prefix rdfs: <http://www.w3.org/2000/01/rdf-schema#> .
@prefix dcterms: <http://purl.org/dc/terms/> .
@prefix foaf: <http://xmlns.com/foaf/spec/> .
@prefix org: <http://www.w3.org/ns/org#> .
@prefix prov: <http://www.w3.org/ns/prov#> .
@prefix xsd: <http://www.w3.org/2001/XMLSchema#> .

# Ontology Metadata
georeference: a owl:Ontology ;
    rdfs:label "Ontology definition for Georeferencing"@en ;
    rdfs:comment "Georeferencing ontology with common classes for location, coordinate reference systems, and spatial properties."@en ;

    dcterms:creator "The GAIA-X 4 PLC AAD Project Team"@en ;
    dcterms:contributor [
        a foaf:Person ;
        foaf:name "Carlo van Driesten" ;
        org:memberOf <https://www.bmwgroup.com/> ;
    ] , [
        a foaf:Person ;
        foaf:name "Sebastian Tuttas" ;
        org:memberOf <https://www.3d-mapping.de/> ;
    ] , [
        a foaf:Person ;
        foaf:name "Mirco Nierenz" ;
        org:memberOf <https://triangraphics.de/> ;
    ] ;  

    # Permanent identifier for the ontology (not version-specific)
    dcterms:identifier <https://ontologies.envited-x.net/georeference> ;

    # GitHub repository where the ontology is maintained
    dcterms:source <https://github.com/GAIA-X4PLC-AAD/ontology-management-base> ;

    # Specific GitHub release used for publishing this version
    prov:wasDerivedFrom <https://github.com/GAIA-X4PLC-AAD/ontology-management-base/releases/tag/v0.0.2> ;

    # Versioning
    owl:versionIRI <https://ontologies.envited-x.net/georeference/v3/ontology> ;
    owl:versionInfo "v3" ;

    # Reference to SHACL validation rules
    dcterms:conformsTo <https://ontologies.envited-x.net/georeference/v3/shape> ;

    # References to related ontologies
    dcterms:references <https://ontologies.envited-x.net/hdmap/v4/ontology> ;
    rdfs:seeAlso <https://github.com/GAIA-X4PLC-AAD/ontology-management-base/blob/main/README.md> .

georeference:Georeference a owl:Class ;
    rdfs:label "Class definition for Georeference"@en ;
    rdfs:comment """A georeferencing dataset that defines the coordinate system, location, and spatial properties of a simulation asset. 
                    This class serves as an optional metadata extension and does not function as a standalone data resource."""@en ;
    rdfs:subClassOf [ 
        a owl:Restriction ; 
        owl:onProperty georeference:hasGeodeticReferenceSystem ; 
        owl:cardinality 1
    ] ;
    rdfs:subClassOf [ 
        a owl:Restriction ; 
        owl:onProperty georeference:hasProjectLocation ; 
        owl:cardinality 1
    ] .

### **Geodetic Reference System**
georeference:GeodeticReferenceSystem a owl:Class ;
    rdfs:label "Class definition for GeodeticReferenceSystem"@en ;
    rdfs:comment "Defines the reference system used to represent coordinates, including projection type and ellipsoid model."@en ;

    # Must have an EPSG code OR a Coordinate System Name
    owl:equivalentClass [
        a owl:Class ;
        owl:unionOf (
            [ a owl:Restriction ; owl:onProperty georeference:codeEPSG ; owl:cardinality 1 ]
            [ a owl:Restriction ; owl:onProperty georeference:coordinateSystemName ; owl:cardinality 1 ]
        )
    ] ;
    rdfs:subClassOf [ 
        a owl:Restriction ; 
        owl:onProperty georeference:hasOrigin ;
        owl:cardinality 1 ;
    ] ;
    rdfs:subClassOf [ 
        a owl:Restriction ; 
        owl:onProperty georeference:hasViewPoint ;
        owl:maxCardinality 1 ;
        owl:someValuesFrom  georeference:LatLonCoordinate 
    ] .

georeference:ProjectLocation a owl:Class ;
    rdfs:label "Class definition for ProjectLocation"@en ;
    rdfs:comment "Contains attributes describing the location of a simulation asset, such as country, region, city, and bounding box."@en ;
    rdfs:subClassOf [ 
        a owl:Restriction ; 
        owl:onProperty georeference:hasBoundingBox ;
        owl:cardinality 1 ;
    ] .

georeference:BoundingBox a owl:Class ;
    rdfs:label "Class definition for BoundingBox"@en ;
    rdfs:comment "Defines a rectangular spatial extent using minimum and maximum values for the x and y axes."@en .

georeference:LatLonCoordinate a owl:Class ;
    rdfs:label "Class definition for LatLonCoordinate"@en ;
    rdfs:comment "Defines world coordinates in latitude and longitude, expressed in degrees."@en .

### **Object Properties**
georeference:hasGeodeticReferenceSystem a owl:ObjectProperty ;
    rdfs:label "has geodetic reference system"@en ;
    rdfs:comment "Links a Georeference to its Geodetic Reference System. REQUIRED (1 per Georeference)."@en ;
    rdfs:domain georeference:Georeference ;
    rdfs:range georeference:GeodeticReferenceSystem .

georeference:hasProjectLocation a owl:ObjectProperty ;
    rdfs:label "has project location"@en ;
    rdfs:comment "Links a Georeference to its Project Location details, which includes the bounding box. REQUIRED (1 per Georeference)."@en ;
    rdfs:domain georeference:Georeference ;
    rdfs:range georeference:ProjectLocation .

georeference:hasBoundingBox a owl:ObjectProperty ;
    rdfs:label "has bounding box"@en ;
    rdfs:comment "Bounding Box is only allowed inside ProjectLocation and defines its spatial extent."@en ;
    rdfs:domain georeference:ProjectLocation ;
    rdfs:range georeference:BoundingBox .

georeference:hasOrigin a owl:ObjectProperty ;
    rdfs:label "has origin"@en ;
    rdfs:comment "Defines the origin position of the asset in world coordinates. REQUIRED."@en ;
    rdfs:domain georeference:GeodeticReferenceSystem ;
    rdfs:range georeference:LatLonCoordinate .
    
georeference:hasViewPoint a owl:ObjectProperty ;
    rdfs:label "has view point"@en ;
    rdfs:comment "Defines the viewpoint position of the asset in world coordinates. OPTIONAL."@en ;
    rdfs:domain georeference:GeodeticReferenceSystem ;
    rdfs:range georeference:LatLonCoordinate .
