@prefix hdmap: <https://w3id.org/ascs-ev/envited-x/hdmap/v5/> .
@prefix envited-x: <https://w3id.org/ascs-ev/envited-x/envited-x/v3/> .
@prefix georeference: <https://w3id.org/ascs-ev/envited-x/georeference/v5/> .
@prefix manifest: <https://w3id.org/ascs-ev/envited-x/manifest/v5/> .
@prefix owl: <http://www.w3.org/2002/07/owl#> .
@prefix dcterms: <http://purl.org/dc/terms/> .
@prefix foaf: <http://xmlns.com/foaf/0.1/> .
@prefix org: <http://www.w3.org/ns/org#> .
@prefix prov: <http://www.w3.org/ns/prov#> .
@prefix rdfs: <http://www.w3.org/2000/01/rdf-schema#> .
@prefix xsd: <http://www.w3.org/2001/XMLSchema#> .
@prefix openlabel: <https://openlabel.asam.net/V1-0-0/ontologies/> .

<https://w3id.org/ascs-ev/envited-x/hdmap/v5> a owl:Ontology ;
    rdfs:label "Ontology definition for hdmap"@en ;
    rdfs:comment "An ontology with common classes to describe a high-definition map (HD map) assets used in simulation."@en ;

    dcterms:creator "The GAIA-X 4 PLC AAD Project Team"@en ;
    dcterms:contributor [
        a foaf:Person ;
        foaf:name "Carlo van Driesten" ;
        org:memberOf <https://www.bmwgroup.com/> ;
    ] , [
        a foaf:Person ;
        foaf:name "Sebastian Tuttas" ;
        org:memberOf <https://www.3d-mapping.de/> ;
    ] , [
        a foaf:Person ;
        foaf:name "Mirco Nierenz" ;
        org:memberOf <https://triangraphics.de/> ;
    ] ;

    # Permanent identifier for the ontology (not version-specific)
    dcterms:identifier <https://w3id.org/ascs-ev/envited-x/hdmap> ;

    # GitHub repository where the ontology is maintained
    dcterms:source <https://github.com/GAIA-X4PLC-AAD/ontology-management-base> ;

    # Specific GitHub release used for publishing this version
    prov:wasDerivedFrom <https://github.com/GAIA-X4PLC-AAD/ontology-management-base/releases/tag/v0.0.5> ;

    # Versioning
    owl:versionIRI <https://w3id.org/ascs-ev/envited-x/hdmap/v5> ;
    owl:versionInfo "v5" ;

    # Imports strict dependencies
    owl:imports <https://w3id.org/ascs-ev/envited-x/envited-x/v3> ,
                <https://w3id.org/ascs-ev/envited-x/georeference/v5> ;

    # Reference to SHACL validation rules
    dcterms:conformsTo <https://w3id.org/ascs-ev/envited-x/hdmap/v5/shapes> ;

    # Additional references to documentation or related ontologies
    dcterms:references <https://www.asam.net/standards/detail/opendrive/> ;
    rdfs:seeAlso <https://ascs-ev.github.io/EVES/> .


#### Classes

hdmap:HdMap a owl:Class ;
    rdfs:label "Class definition for HdMap"@en ;
    rdfs:comment "General properties for defining a high-definition map (HD map) asset used in simulation environments, such as format, content, quantity and quality properties."@en ;
    rdfs:subClassOf envited-x:SimulationAsset ;
    rdfs:subClassOf [
        a owl:Restriction ;
        owl:onProperty hdmap:hasDomainSpecification ;
        owl:someValuesFrom hdmap:DomainSpecification
    ] ;
    rdfs:subClassOf [
        a owl:Restriction ;
        owl:onProperty hdmap:hasResourceDescription ;
        owl:someValuesFrom [
            a owl:Class ;
            owl:unionOf ( envited-x:ResourceDescription manifest:Link )
        ]
    ] ;
    rdfs:subClassOf [
        a owl:Restriction ;
        owl:onProperty hdmap:hasManifest ;
        owl:someValuesFrom [
            a owl:Class ;
            owl:unionOf ( envited-x:Manifest manifest:Link )
        ]
    ] .

hdmap:DomainSpecification a owl:Class ;
    rdfs:label "Class definition for DomainSpecification"@en ;
    rdfs:comment "HD map DomainSpecification containing additional metadata information of the simulation asset."@en ;
    rdfs:subClassOf envited-x:DomainSpecification ;
    rdfs:subClassOf [
        a owl:Restriction ;
        owl:onProperty hdmap:hasContent ;
        owl:minCardinality 1
    ] , [
        a owl:Restriction ;
        owl:onProperty hdmap:hasDataSource ;
        owl:cardinality 1
    ] , [
        a owl:Restriction ;
        owl:onProperty hdmap:hasFormat ;
        owl:cardinality 1
    ] , [
        a owl:Restriction ;
        owl:onProperty hdmap:hasQuality ;
        owl:cardinality 1
    ] , [
        a owl:Restriction ;
        owl:onProperty hdmap:hasQuantity ;
        owl:cardinality 1
    ] , [
        a owl:Restriction ;
        owl:onProperty hdmap:hasGeoreference ;
        owl:cardinality 1
    ] .

hdmap:Content a owl:Class ;
    rdfs:label "Class definition for Content"@en ;
    rdfs:comment "Defines the content (road types, lane types, object types, traffic direction) of the HD map asset."@en ;
    rdfs:subClassOf envited-x:Content .

hdmap:DataSource a owl:Class ;
    rdfs:label "Class definition for DataSource"@en ;
    rdfs:comment "Defines which data resources or measurement systems were used to create the HD map asset."@en ;
    rdfs:subClassOf envited-x:DataSource .

hdmap:Format a owl:Class ;
    rdfs:label "Class definition for Format"@en ;
    rdfs:comment "Contains properties to describe the format of the HD map asset."@en ;
    rdfs:subClassOf envited-x:Format .

hdmap:Quality a owl:Class ;
    rdfs:label "Class definition for Quality"@en ;
    rdfs:comment "Contains properties to describe the accuracy of the HD map asset."@en ;
    rdfs:subClassOf envited-x:Quality ;
    rdfs:subClassOf [
        a owl:Restriction ;
        owl:onProperty hdmap:hasRange2D ;
        owl:someValuesFrom hdmap:Range2D
    ] .

hdmap:Quantity a owl:Class ;
    rdfs:label "Class definition for Quantity"@en ;
    rdfs:comment "Contains properties to describe the quantity (e.g. number of intersections, traffic lights, signs, length, range of speed limits/elevations) of the HD map asset."@en ;
    rdfs:subClassOf envited-x:Quantity .

# Used in Quantity
hdmap:Range2D a owl:Class ;
    rdfs:label "Class definition for Range2D"@en ;
    rdfs:comment "Range2D definition with minimum to maximum data property usable in the HD map asset."@en .


#### Object properties

### hasDomainSpecification (HdMap -> DomainSpecification)
hdmap:hasDomainSpecification a owl:ObjectProperty ;
    rdfs:label "Object property: hasDomainSpecification"@en ;
    rdfs:comment "Links an HD map asset to its specific metadata (DomainSpecification), which may contain additional HD map-specific attributes."@en ;
    rdfs:subPropertyOf envited-x:hasDomainSpecification ;
    rdfs:domain hdmap:HdMap ;
    rdfs:range hdmap:DomainSpecification .

### hasResourceDescription (HdMap -> envited-x:ResourceDescription)
hdmap:hasResourceDescription a owl:ObjectProperty ;
    rdfs:label "Object property: hasResourceDescription"@en ;
    rdfs:comment "Links an HD map asset to a standard ResourceDescription instance from envited-x."@en ;
    rdfs:subPropertyOf envited-x:hasResourceDescription ;
    rdfs:domain hdmap:HdMap ;
    rdfs:range [
        a owl:Class ;
        owl:unionOf ( envited-x:ResourceDescription manifest:Link )
    ] .

### hasManifest (HdMap -> envited-x:Manifest OR manifest:Link)
hdmap:hasManifest a owl:ObjectProperty ;
    rdfs:label "Object property: hasManifest"@en ;
    rdfs:comment """
                Links an HD map asset to its manifest.
                The value can be either:
                - an inline envited-x:Manifest node (embedded manifest structure), or
                - an manifest:Link node (a link that points via manifest:iri
                to an external manifest representation, typically identified by a DID).
                """@en ;
    rdfs:subPropertyOf envited-x:hasManifest ;
    rdfs:domain hdmap:HdMap ;
    rdfs:range [
        a owl:Class ;
        owl:unionOf ( envited-x:Manifest manifest:Link )
    ] .

# Union class for HDMap Content or OpenLABEL OddScenery
hdmap:ContentOrOddScenery a owl:Class ;
    rdfs:label "Content or OpenLabel OddScenery"@en ;
    rdfs:comment "Combines HDMap content with OpenLABEL's OddScenery."@en ;
    owl:unionOf (hdmap:Content openlabel:OddScenery) .

### hasContent (DomainSpecification -> Content)
hdmap:hasContent a owl:ObjectProperty ;
    rdfs:label "Object property: hasContent"@en ;
    rdfs:comment "Links a DomainSpecification to an instance of hdmap:Content that describes the HD map`s content."@en ;
    rdfs:subPropertyOf envited-x:hasContent ;
    rdfs:domain hdmap:DomainSpecification ;
    rdfs:range hdmap:ContentOrOddScenery .

### hasDataSource (DomainSpecification -> DataSource)
hdmap:hasDataSource a owl:ObjectProperty ;
    rdfs:label "Object property: hasDataSource"@en ;
    rdfs:comment "Links a DomainSpecification to an instance of hdmap:DataSource that describes how the HD map was created."@en ;
    rdfs:subPropertyOf envited-x:hasDataSource ;
    rdfs:domain hdmap:DomainSpecification ;
    rdfs:range hdmap:DataSource .

### hasFormat (DomainSpecification -> Format)
hdmap:hasFormat a owl:ObjectProperty ;
    rdfs:label "Object property: hasFormat"@en ;
    rdfs:comment "Links a DomainSpecification to an instance of hdmap:Format that describes the HD map`s format details."@en ;
    rdfs:subPropertyOf envited-x:hasFormat ;
    rdfs:domain hdmap:DomainSpecification ;
    rdfs:range hdmap:Format .

### hasQuality (DomainSpecification -> Quality)
hdmap:hasQuality a owl:ObjectProperty ;
    rdfs:label "Object property: hasQuality"@en ;
    rdfs:comment "Links a DomainSpecification to an instance of hdmap:Quality describing the HD map`s quality or accuracy aspects."@en ;
    rdfs:subPropertyOf envited-x:hasQuality ;
    rdfs:domain hdmap:DomainSpecification ;
    rdfs:range hdmap:Quality .

### hasQuantity (DomainSpecification -> Quantity)
hdmap:hasQuantity a owl:ObjectProperty ;
    rdfs:label "Object property: hasQuantity"@en ;
    rdfs:comment "Links a DomainSpecification to an instance of hdmap:Quantity describing the HD map`s quantity (intersections, traffic signs, etc.)."@en ;
    rdfs:subPropertyOf envited-x:hasQuantity ;
    rdfs:domain hdmap:DomainSpecification ;
    rdfs:range hdmap:Quantity .

### hasRange2D (DomainSpecification -> Range2D)
hdmap:hasRange2D a owl:ObjectProperty ;
    rdfs:label "Object property: hasRange2D"@en ;
    rdfs:comment "Links a DomainSpecification to an instance of hdmap:Range2D describing the 2D bounding area of the HD map asset."@en ;
    rdfs:domain hdmap:DomainSpecification ;
    rdfs:range hdmap:Range2D .

### hasGeoreference (DomainSpecification -> georeference:Georeference)
hdmap:hasGeoreference a owl:ObjectProperty ;
    rdfs:label "Object property: hasGeoreference"@en ;
    rdfs:comment "Links a DomainSpecification to a georeference:Georeference describing how the HD map is georeferenced."@en ;
    rdfs:domain hdmap:DomainSpecification ;
    rdfs:range georeference:Georeference .
