@prefix manifest: <https://github.com/GAIA-X4PLC-AAD/ontology-management-base/tree/main/manifest/> .
@prefix owl: <http://www.w3.org/2002/07/owl#> .
@prefix dcterms: <http://purl.org/dc/terms/> .
@prefix foaf: <http://xmlns.com/foaf/spec/> .
@prefix org: <http://www.w3.org/ns/org#> .
@prefix prov: <http://www.w3.org/ns/prov#> .
@prefix rdfs: <http://www.w3.org/2000/01/rdf-schema#> .
@prefix gx: <https://registry.lab.gaia-x.eu/development/api/trusted-shape-registry/v1/shapes/jsonld/trustframework#> .
@prefix xsd: <http://www.w3.org/2001/XMLSchema#> .

manifest: a owl:Ontology ;
    rdfs:label "Ontology definition for manifest"@en ;
    rdfs:comment "An ontology with common classes to describe the structure as list of contents of a domain specific asset using a manifest.json e.g. in an archive."@en ;

    dcterms:creator "The GAIA-X 4 PLC AAD Project Team"@en ;
    dcterms:contributor [
        a foaf:Person ;
        foaf:name "Johannes Demer" ;
        org:memberOf <https://www.asc-s.de/> ;
    ] , [
        a foaf:Person ;
        foaf:name "Carlo van Driesten" ;
        org:memberOf <https://www.bmwgroup.com/> ;
    ] , [
        a foaf:Person ;
        foaf:name "Mirco Nierenz" ;
        org:memberOf <https://triangraphics.de/> ;
    ] , [
        a foaf:Person ;
        foaf:name "Erik Konietzko" ;
        org:memberOf <https://www.ipk.fraunhofer.de/> ;
    ] ;

    # Permanent identifier for the ontology (not version-specific)
    dcterms:identifier <https://ontologies.envited-x.net/manifest> ;

    # GitHub repository where the ontology is maintained
    dcterms:source <https://github.com/GAIA-X4PLC-AAD/ontology-management-base> ;

    # Specific GitHub release used for publishing this version
    prov:wasDerivedFrom <https://github.com/GAIA-X4PLC-AAD/ontology-management-base/releases/tag/v0.0.2> ;

    # Versioning
    owl:versionIRI <https://ontologies.envited-x.net/manifest/v3/ontology> ;
    owl:versionInfo "v3" ;

    # Reference to SHACL validation rules
    dcterms:conformsTo <https://ontologies.envited-x.net/manifest/v3/shape> ;

    # Additional references to the ENVITED Ecosystem Specification (EVES) or related ontologies
    dcterms:references <https://ontologies.envited-x.net/envited-x/v1/ontology> ;
    rdfs:seeAlso <https://ascs-ev.github.io/EVES/> .

manifest:Manifest a owl:Class ;
    rdfs:label "Class definition for Manifest"@en ;
    rdfs:comment "Defines the structure as list of contents of an asset (e.g. simulation asset) using a manifest.json, including content data and license as linked properties."@en .

manifest:License a owl:Class ;
    rdfs:label "Class definition for License"@en ;
    rdfs:comment "General class for defining the license of an asset."@en .

### Define Link class with restriction on FileMetaData
manifest:Link a owl:Class ;
    rdfs:label "Class definition for Link"@en ;
    rdfs:comment "General class for defining a link to data within an archive, related published simulation assets, or other web references."@en ;
    rdfs:subClassOf [
        a owl:Restriction ;
        owl:onProperty manifest:fileMetaData ;
        owl:someValuesFrom manifest:FileMetaData
    ] .

### Restrict FileMetaData to only be used inside manifest:Link
manifest:FileMetaData a owl:Class ;
    rdfs:label "Class definition for FileMetaData"@en ;
    rdfs:comment "General class for defining the properties of a data file referenced inside a manifest:Link."@en ;
    rdfs:subClassOf manifest:Link ;
    rdfs:subClassOf [
        a owl:Restriction ;
        owl:onProperty manifest:dimensions ;
        owl:someValuesFrom manifest:Dimensions
    ] .

### Restrict Dimensions to only be used inside FileMetaData
manifest:Dimensions a owl:Class ;
    rdfs:label "Class definition for Dimensions"@en ;
    rdfs:comment "General class for defining the dimensions of a data file, e.g., of type image or video, referenced inside a manifest:FileMetaData."@en ;
    rdfs:subClassOf manifest:FileMetaData .
