@prefix manifest: <https://github.com/GAIA-X4PLC-AAD/ontology-management-base/tree/main/manifest/> .
@prefix owl: <http://www.w3.org/2002/07/owl#> .
@prefix dcterms: <http://purl.org/dc/terms/> .
@prefix foaf: <http://xmlns.com/foaf/spec/> .
@prefix org: <http://www.w3.org/ns/org#> .
@prefix prov: <http://www.w3.org/ns/prov#> .
@prefix rdfs: <http://www.w3.org/2000/01/rdf-schema#> .
@prefix gx: <https://registry.lab.gaia-x.eu/development/api/trusted-shape-registry/v1/shapes/jsonld/trustframework#> .
@prefix xsd: <http://www.w3.org/2001/XMLSchema#> .

manifest: a owl:Ontology ;
    rdfs:label "Ontology definition for manifest"@en ;
    rdfs:comment "An ontology with common classes to describe the structure as list of contents of a domain specific asset using a manifest.json e.g. in an archive."@en ;

    dcterms:creator "The GAIA-X 4 PLC AAD Project Team"@en ;
    dcterms:contributor [
        a foaf:Person ;
        foaf:name "Johannes Demer" ;
        org:memberOf <https://www.asc-s.de/> ;
    ] , [
        a foaf:Person ;
        foaf:name "Carlo van Driesten" ;
        org:memberOf <https://www.bmwgroup.com/> ;
    ] , [
        a foaf:Person ;
        foaf:name "Mirco Nierenz" ;
        org:memberOf <https://triangraphics.de/> ;
    ] , [
        a foaf:Person ;
        foaf:name "Erik Konietzko" ;
        org:memberOf <https://www.ipk.fraunhofer.de/> ;
    ] ;

    # Permanent identifier for the ontology (not version-specific)
    dcterms:identifier <https://ontologies.envited-x.net/manifest> ;

    # GitHub repository where the ontology is maintained
    dcterms:source <https://github.com/GAIA-X4PLC-AAD/ontology-management-base> ;

    # Specific GitHub release used for publishing this version
    prov:wasDerivedFrom <https://github.com/GAIA-X4PLC-AAD/ontology-management-base/releases/tag/v0.0.2> ;

    # Versioning
    owl:versionIRI <https://ontologies.envited-x.net/manifest/v3/ontology> ;
    owl:versionInfo "v3" ;

    # Reference to SHACL validation rules
    dcterms:conformsTo <https://ontologies.envited-x.net/manifest/v3/shape> ;

    # Additional references to the ENVITED Ecosystem Specification (EVES) or related ontologies
    dcterms:references <https://ontologies.envited-x.net/envited-x/v1/ontology> ;
    rdfs:seeAlso <https://ascs-ev.github.io/EVES/> .


manifest:Manifest a owl:Class ;
    rdfs:label "Class definition for Manifest"@en ;
    rdfs:comment "Defines the structure as list of contents of an asset (e.g. simulation asset) using a manifest.json, including content data and license as linked properties."@en ;
    rdfs:subClassOf [ 
        a owl:Restriction ; 
        owl:onProperty manifest:hasManifestReference ; 
        owl:cardinality 1
    ] ;
    rdfs:subClassOf [ 
        a owl:Restriction ; 
        owl:onProperty manifest:hasLicense ; 
        owl:cardinality 1
    ] ;
    rdfs:subClassOf [ 
        a owl:Restriction ; 
        owl:onProperty manifest:hasArtifacts ;  
        owl:someValuesFrom manifest:Link
    ] ;
    rdfs:subClassOf [ 
        a owl:Restriction ; 
        owl:onProperty manifest:hasReferencedArtifacts ;  
        owl:minCardinality 0
    ] .


manifest:Link a owl:Class ;
    rdfs:label "Class definition for Link"@en ;
    rdfs:comment "Defines a Link instance that connects to data and mandatory metadata within an archive or related published simulation assets; can include web references."@en ;
    rdfs:subClassOf [
        a owl:Restriction ;
        owl:onProperty manifest:hasFileMetadata ;
        owl:cardinality 1
    ] .


manifest:FileMetadata a owl:Class ;
    rdfs:label "Class definition for FileMetadata"@en ;
    rdfs:comment "Represents the properties of a data file referenced within a Link instance."@en ;
    rdfs:subClassOf [ 
        a owl:Restriction ; 
        owl:onProperty manifest:hasDimensions ;  
        owl:minCardinality 0
    ] .


manifest:License a owl:Class ;
    rdfs:label "Class definition for License"@en ;
    rdfs:comment "General subclass of Link for defining the license of an asset."@en .


manifest:Dimensions a owl:Class ;
    rdfs:label "Class definition for Dimensions"@en ;
    rdfs:comment "General class for defining the dimensions of a data file, e.g., of type image or video, referenced inside a manifest:FileMetadata."@en .


# Object properties
manifest:hasManifestReference a owl:ObjectProperty ;
    rdfs:domain manifest:Manifest ;
    rdfs:range manifest:Link ;
    rdfs:comment "Links a Manifest to its corresponding manifest reference file, defining the structure and contents of a digital asset; only applicable within Manifest instances."@en .


manifest:hasLicense a owl:ObjectProperty ;
    rdfs:domain manifest:Manifest ;
    rdfs:range manifest:License ;
    rdfs:comment "Associates a Manifest instance with its corresponding License; only applicable within Manifest instances."@en .


manifest:hasArtifacts a owl:ObjectProperty ;
    rdfs:domain manifest:Manifest ;
    rdfs:range manifest:Link ;
    rdfs:comment "Associates a Manifest instance with its artifacts, represented as Link instances; only applicable within Manifest instances."@en .


manifest:hasReferencedArtifacts a owl:ObjectProperty ;
    rdfs:domain manifest:Manifest ;
    rdfs:range manifest:Link ;
    rdfs:comment "Associates a Manifest instance with its external artifacts, represented as Link instances; only applicable within Manifest instances."@en .


manifest:hasFileMetadata a owl:ObjectProperty ;
    rdfs:domain manifest:Link ;
    rdfs:range manifest:FileMetadata ;
    rdfs:comment "Associates a FileMetadata instance with its corresponding Link; only applicable within Link instances."@en .


manifest:hasDimensions a owl:ObjectProperty ;
    rdfs:domain manifest:FileMetadata ;
    rdfs:range manifest:Dimensions ;
    rdfs:comment "Links a Dimensions instance to its associated FileMetadata, defining the size and scale of the data file; applicable only within FileMetadata instances."@en .

## Define a general access role class
manifest:AccessRole a owl:Class ;
    rdfs:label "AccessRole"@en ;
    rdfs:comment "A class representing different access roles of artifacts in a manifest."@en .

## General accessRole property
manifest:hasAccessRole a owl:ObjectProperty ;
    rdfs:label "has AccessRole"@en ;
    rdfs:comment "General property to indicate the access role of an artifact."@en ;
    rdfs:domain manifest:Link ;
    rdfs:range manifest:AccessRole .

## Define specific access role types as named individuals (NOT subclasses)
manifest:isPublic a manifest:AccessRole, owl:NamedIndividual ;
    rdfs:label "Public Access Role"@en ;
    rdfs:comment "Indicates that the artifact access role is public."@en .

## Define a general category class
manifest:Category a owl:Class ;
    rdfs:label "Category"@en ;
    rdfs:comment "A class representing different categories of artifacts in a manifest."@en .

## General category property
manifest:hasCategory a owl:ObjectProperty ;
    rdfs:label "has Category"@en ;
    rdfs:comment "General property to indicate the category of an artifact."@en ;
    rdfs:domain manifest:Link ;
    rdfs:range manifest:Category .

## Define specific category types as named individuals (NOT subclasses)
manifest:isManifest a manifest:Category, owl:NamedIndividual ;
    rdfs:label "Manifest Category"@en ;
    rdfs:comment "Indicates that the artifact category is a manifest."@en .

manifest:isLicense a manifest:Category, owl:NamedIndividual ;
    rdfs:label "License Category"@en ;
    rdfs:comment "Indicates that the artifact category is a license file."@en .

manifest:isMiscellaneous a manifest:Category, owl:NamedIndividual ;
    rdfs:label "Miscellaneous Category"@en ;
    rdfs:comment "Indicates that the artifact category is miscellaneous."@en .
