@prefix vv-report: <https://w3id.org/gaia-x4plcaad/ontologies/vv-report/v2/> .
@prefix dcterms: <http://purl.org/dc/terms/> .
@prefix foaf: <http://xmlns.com/foaf/0.1/> .
@prefix org: <http://www.w3.org/ns/org#> .
@prefix prov: <http://www.w3.org/ns/prov#> .
@prefix owl: <http://www.w3.org/2002/07/owl#> .
@prefix rdfs: <http://www.w3.org/2000/01/rdf-schema#> .
@prefix xsd: <http://www.w3.org/2001/XMLSchema#> .
@prefix gx: <https://w3id.org/gaia-x/development#> .
@prefix general: <https://w3id.org/gaia-x4plcaad/ontologies/general/v3/> .

<https://w3id.org/gaia-x4plcaad/ontologies/vv-report/v2> a owl:Ontology ;
    rdfs:label "Ontology definition for vv-report"@en ;
    rdfs:comment "An ontology with common classes to describe the structure of a verification & validation report."@en ;
    
    dcterms:contributor [
        a foaf:Person ;
        foaf:name "Maurizio Ahmann" ;
        org:memberOf <https://www.setlabs.de/> ;
    ] , [
        a foaf:Person ;
        foaf:name "Carlo van Driesten" ;
        org:memberOf <https://www.bmwgroup.com/> ;
    ] ;  

    # Permanent identifier for the ontology (not version-specific)
    dcterms:identifier <https://w3id.org/gaia-x4plcaad/ontologies/vv-report> ;

    # GitHub repository where the ontology is maintained
    dcterms:source <https://github.com/GAIA-X4PLC-AAD/ontology-management-base> ;

    # Specific GitHub release used for publishing this version
    prov:wasDerivedFrom <https://github.com/GAIA-X4PLC-AAD/ontology-management-base/releases/tag/v0.0.5> ;

    # Versioning
    owl:versionIRI <https://w3id.org/gaia-x4plcaad/ontologies/vv-report/v2> ;
    owl:versionInfo "v2" ;

    # Reference to SHACL validation rules
    dcterms:conformsTo <https://w3id.org/gaia-x4plcaad/ontologies/vv-report/v2/shapes> ;

    # Additional references to the ENVITED Ecosystem Specification (EVES) or related ontologies
    dcterms:references <https://github.com/asam-ev/qc-framework> ;
    rdfs:seeAlso <https://github.com/GAIA-X4PLC-AAD/ontology-management-base/blob/main/README.md> .

# Classes

vv-report:VvReport a owl:Class ;
    rdfs:label "Class definition for VvReport"@en ;
    rdfs:comment "Attributes for a verification & validation report."@en ;
    rdfs:subClassOf gx:DataResource .

vv-report:Evaluation a owl:Class ;
    rdfs:label "Class definition for Evaluation"@en ;
    rdfs:comment "Attributes for an evaluation element of a verification & validation report."@en .

vv-report:Metric a owl:Class ;
    rdfs:label "Class definition for Metric"@en ;
    rdfs:comment "Attributes for the definition of a quality metric of a verification & validation report."@en .

vv-report:InputData a owl:Class ;
    rdfs:label "Class definition for InputData"@en ;
    rdfs:comment "Attributes for the definition of an input data element of a verification & validation report."@en .

vv-report:Parameter a owl:Class ;
    rdfs:label "Class definition for Parameter"@en ;
    rdfs:comment "Attributes for the definition of parameter element of a verification & validation report."@en .

vv-report:Result a owl:Class ;
    rdfs:label "Class definition for Result"@en ;
    rdfs:comment "Attributes for evaluation results of a verification & validation report."@en .

vv-report:ResultVerification a owl:Class ;
    rdfs:label "Class definition for ResultVerification"@en ;
    rdfs:comment "Attributes for the verification of the result by a third party of a verification & validation report."@en .

# Properties

vv-report:general a owl:ObjectProperty ;
    rdfs:label "general"@en ;
    rdfs:comment "General object with properties for descriptions, data, links, bundle."@en ;
    rdfs:domain vv-report:VvReport ;
    rdfs:range general:General .

vv-report:systemUnderTest a owl:DatatypeProperty ;
    rdfs:label "system under test"@en ;
    rdfs:comment "Uniform Resource Identifier (URI) to identify the tested artifact."@en ;
    rdfs:domain vv-report:VvReport ;
    rdfs:range xsd:anyURI .

vv-report:evaluations a owl:ObjectProperty ;
    rdfs:label "evaluations"@en ;
    rdfs:comment "A list of all measures carried out on the subject under test."@en ;
    rdfs:domain vv-report:VvReport ;
    rdfs:range vv-report:Evaluation .

vv-report:metric a owl:ObjectProperty ;
    rdfs:label "metric"@en ;
    rdfs:comment "The definition of the quality metric that has been used in this evaluation item."@en ;
    rdfs:domain vv-report:Evaluation ;
    rdfs:range vv-report:Metric .

vv-report:inputData a owl:ObjectProperty ;
    rdfs:label "input data"@en ;
    rdfs:comment "The definition of a dataset that has been used as input to the quality metric."@en ;
    rdfs:domain vv-report:Evaluation ;
    rdfs:range vv-report:InputData .

vv-report:parameters a owl:ObjectProperty ;
    rdfs:label "parameters"@en ;
    rdfs:comment "A list of parameters that have been used to configure the quality metric and/or quality criterion."@en ;
    rdfs:domain vv-report:Evaluation ;
    rdfs:range vv-report:Parameter .

vv-report:result a owl:ObjectProperty ;
    rdfs:label "result"@en ;
    rdfs:comment "The summary of the result of this evaluation item."@en ;
    rdfs:domain vv-report:Evaluation ;
    rdfs:range vv-report:Result .

vv-report:conceptSpecificData a owl:ObjectProperty ;
    rdfs:label "concept specific data"@en ;
    rdfs:comment "Additional arbitrary V&V-concept specific data, to further describe the evaluation."@en ;
    rdfs:domain vv-report:Evaluation .

vv-report:metricTitle a owl:DatatypeProperty ;
    rdfs:label "metric title"@en ;
    rdfs:comment "A meaningful name of this metric."@en ;
    rdfs:domain vv-report:Metric ;
    rdfs:range xsd:string .

vv-report:metricDescription a owl:DatatypeProperty ;
    rdfs:label "metric description"@en ;
    rdfs:comment "A short description of what is tested within this quality metric."@en ;
    rdfs:domain vv-report:Metric ;
    rdfs:range xsd:string .

vv-report:metricReference a owl:DatatypeProperty ;
    rdfs:label "metric reference"@en ;
    rdfs:comment "URI to identify the metric."@en ;
    rdfs:domain vv-report:Metric ;
    rdfs:range xsd:anyURI .

vv-report:inputDescription a owl:DatatypeProperty ;
    rdfs:label "input description"@en ;
    rdfs:comment "A short description for interpreting this input data element."@en ;
    rdfs:domain vv-report:InputData ;
    rdfs:range xsd:string .

vv-report:inputReference a owl:DatatypeProperty ;
    rdfs:label "input reference"@en ;
    rdfs:comment "URI to identify the utilized input data element."@en ;
    rdfs:domain vv-report:InputData ;
    rdfs:range xsd:anyURI .

vv-report:parameterName a owl:DatatypeProperty ;
    rdfs:label "parameter name"@en ;
    rdfs:comment "The formal name of the parameter."@en ;
    rdfs:domain vv-report:Parameter ;
    rdfs:range xsd:string .

vv-report:parameterDescription a owl:DatatypeProperty ;
    rdfs:label "parameter description"@en ;
    rdfs:comment "A short description of the parameter."@en ;
    rdfs:domain vv-report:Parameter ;
    rdfs:range xsd:string .

vv-report:parameterValue a owl:DatatypeProperty ;
    rdfs:label "parameter value"@en ;
    rdfs:comment "The value of the parameter."@en ;
    rdfs:domain vv-report:Parameter .

vv-report:resultTestPassed a owl:DatatypeProperty ;
    rdfs:label "result test passed"@en ;
    rdfs:comment "Statement if the test has been passed or not."@en ;
    rdfs:domain vv-report:Result ;
    rdfs:range xsd:boolean .

vv-report:resultLog a owl:DatatypeProperty ;
    rdfs:label "result log"@en ;
    rdfs:comment "Additional information about the test result."@en ;
    rdfs:domain vv-report:Result ;
    rdfs:range xsd:string .

vv-report:resultVerifiable a owl:DatatypeProperty ;
    rdfs:label "result verifiable"@en ;
    rdfs:comment "Information if the result can be verified by a third party."@en ;
    rdfs:domain vv-report:Result ;
    rdfs:range xsd:boolean .

vv-report:resultVerification a owl:ObjectProperty ;
    rdfs:label "result verification"@en ;
    rdfs:comment "The necessary attributes to carry out verification of the result by a third party."@en ;
    rdfs:domain vv-report:Result ;
    rdfs:range vv-report:ResultVerification .

vv-report:resultVerificationDescription a owl:DatatypeProperty ;
    rdfs:label "result verification description"@en ;
    rdfs:comment "A short description of how the result can be verified."@en ;
    rdfs:domain vv-report:ResultVerification ;
    rdfs:range xsd:string .

vv-report:resultVerificationReference a owl:DatatypeProperty ;
    rdfs:label "result verification reference"@en ;
    rdfs:comment "URI to identify the reference used to verify the result."@en ;
    rdfs:domain vv-report:ResultVerification ;
    rdfs:range xsd:anyURI .
