@prefix surface-model: <https://ontologies.envited-x.net/surface-model/v6/ontology#> .
@prefix envited-x: <https://ontologies.envited-x.net/envited-x/v3/ontology#> .
@prefix manifest: <https://ontologies.envited-x.net/manifest/v5/ontology#> .
@prefix georeference: <https://ontologies.envited-x.net/georeference/v5/ontology#> .
@prefix dcterms: <http://purl.org/dc/terms/> .
@prefix foaf: <http://xmlns.com/foaf/0.1/> .
@prefix org: <http://www.w3.org/ns/org#> .
@prefix prov: <http://www.w3.org/ns/prov#> .
@prefix owl: <http://www.w3.org/2002/07/owl#> .
@prefix rdfs: <http://www.w3.org/2000/01/rdf-schema#> .
@prefix xsd: <http://www.w3.org/2001/XMLSchema#> .
@prefix gx: <https://w3id.org/gaia-x/development/> .


surface-model: a owl:Ontology ;
    rdfs:label "Ontology definition for surface-model"@en ;
    rdfs:comment "An ontology with common classes used to describe a surface-model asset."@en ;

    dcterms:creator "The GAIA-X 4 PLC AAD Project Team"@en ;
    dcterms:contributor [
        a foaf:Person ;
        foaf:name "Sebastian Tuttas" ;
        org:memberOf <https://www.3d-mapping.de/> ;
    ] , [
        a foaf:Person ;
        foaf:name "Mirco Nierenz" ;
        org:memberOf <https://triangraphics.de/> ;
    ] , [
        a foaf:Person ;
        foaf:name "Carlo van Driesten" ;
        org:memberOf <https://www.bmwgroup.com/> ;
    ] ;

    # Permanent identifier for the ontology (not version-specific)
    dcterms:identifier <https://ontologies.envited-x.net/surface-model> ;

    # GitHub repository where the ontology is maintained
    dcterms:source <https://github.com/GAIA-X4PLC-AAD/ontology-management-base> ;

    # Specific GitHub release used for publishing this version
    prov:wasDerivedFrom <https://github.com/GAIA-X4PLC-AAD/ontology-management-base/releases/tag/v0.0.5> ;

    # Versioning
    owl:versionIRI <https://ontologies.envited-x.net/surface-model/v6/ontology#> ;
    owl:versionInfo "v6" ;

    # Reference to SHACL validation rules
    dcterms:conformsTo <https://ontologies.envited-x.net/surface-model/v6/shape#> ;

    # Additional references to the ENVITED Ecosystem Specification (EVES) or related ontologies
    dcterms:references <https://www.asam.net/standards/detail/opencrg/> ;
    rdfs:seeAlso <https://ascs-ev.github.io/EVES/> .

surface-model:SurfaceModel a owl:Class ;
    rdfs:label "Class definition for SurfaceModel"@en ;
    rdfs:comment "General properties for defining a surface model asset, including format, content, data sources, quantity, and quality attributes."@en ;
    rdfs:subClassOf envited-x:SimulationAsset ;
    rdfs:subClassOf [
        a owl:Restriction ;
        owl:onProperty surface-model:hasDataResourceExtension ;
        owl:someValuesFrom surface-model:DataResourceExtension
    ] ;
    rdfs:subClassOf [
        a owl:Restriction ;
        owl:onProperty surface-model:hasDataResource ;
        owl:someValuesFrom [
            a owl:Class ;
            owl:unionOf ( envited-x:DataResource manifest:Link )
        ]
    ] ;
    rdfs:subClassOf [
        a owl:Restriction ;
        owl:onProperty surface-model:hasManifest ;
        owl:someValuesFrom [
            a owl:Class ;
            owl:unionOf ( envited-x:Manifest manifest:Link )
        ]
    ] .

surface-model:DataResourceExtension a owl:Class ;
    rdfs:label "Class definition for DataResourceExtension"@en ;
    rdfs:comment "Surface model DataResourceExtension containing additional metadata information of the simulation asset."@en ;
    rdfs:subClassOf envited-x:DataResourceExtension ;
    rdfs:subClassOf [
        a owl:Restriction ;
        owl:onProperty surface-model:hasContent ;
        owl:cardinality 1
    ] , [
        a owl:Restriction ;
        owl:onProperty surface-model:hasFormat ;
        owl:cardinality 1
    ] , [
        a owl:Restriction ;
        owl:onProperty surface-model:hasQuality ;
        owl:cardinality 1
    ] , [
        a owl:Restriction ;
        owl:onProperty surface-model:hasQuantity ;
        owl:cardinality 1
    ] , [
        a owl:Restriction ;
        owl:onProperty surface-model:hasGeoreference ;
        owl:cardinality 1
    ] .

surface-model:Content a owl:Class ;
    rdfs:label "Class definition for Content"@en ;
    rdfs:comment "Contains properties that describe the content type of the surface model asset."@en ;
    rdfs:subClassOf envited-x:Content .

surface-model:Format a owl:Class ;
    rdfs:label "Class definition for Format"@en ;
    rdfs:comment "Contains properties that describe the format of the surface model asset."@en ;
    rdfs:subClassOf envited-x:Format .

surface-model:Quality a owl:Class ;
    rdfs:label "Class definition for Quality"@en ;
    rdfs:comment "Contains properties that describe the accuracy of the surface model asset."@en ;
    rdfs:subClassOf envited-x:Quality .

surface-model:Quantity a owl:Class ;
    rdfs:label "Class definition for Quantity"@en ;
    rdfs:comment "Contains properties that describe the quantity of the surface model asset."@en ;
    rdfs:subClassOf envited-x:Quantity .


### Object Properties

surface-model:hasDataResourceExtension a owl:ObjectProperty ;
    rdfs:label "Object property: hasDataResourceExtension"@en ;
    rdfs:comment "Links a surface model asset to its specific metadata (DataResourceExtension), which may contain additional surface model-specific attributes."@en ;
    rdfs:subPropertyOf envited-x:hasDataResourceExtension ;
    rdfs:domain surface-model:SurfaceModel ;
    rdfs:range surface-model:DataResourceExtension .

surface-model:hasDataResource a owl:ObjectProperty ;
    rdfs:label "Object property: hasDataResource"@en ;
    rdfs:comment "Links a surface model asset to a standard DataResource instance from envited-x."@en ;
    rdfs:subPropertyOf envited-x:hasDataResource ;
    rdfs:domain surface-model:SurfaceModel ;
    rdfs:range [
        a owl:Class ;
        owl:unionOf ( envited-x:DataResource manifest:Link )
    ] .

surface-model:hasManifest a owl:ObjectProperty ;
    rdfs:label "Object property: hasManifest"@en ;
    rdfs:comment "Links a surface model asset to its manifest. May be inline or via link."@en ;
    rdfs:subPropertyOf envited-x:hasManifest ;
    rdfs:domain surface-model:SurfaceModel ;
    rdfs:range [
        a owl:Class ;
        owl:unionOf ( envited-x:Manifest manifest:Link )
    ] .


surface-model:hasGeoreference a owl:ObjectProperty ;
    rdfs:label "Object property: hasGeoreference"@en ;
    rdfs:comment "Links a DataResourceExtension to a georeference:Georeference describing how the surface model is georeferenced."@en ;
    rdfs:domain surface-model:DataResourceExtension ;
    rdfs:range georeference:Georeference .

surface-model:hasContent a owl:ObjectProperty ;
    rdfs:label "Object property: hasContent"@en ;
    rdfs:comment "Links a DataResourceExtension to an instance of surface-model:Content that describes the surface model's data content."@en ;
    rdfs:subPropertyOf envited-x:hasContent ;
    rdfs:domain surface-model:DataResourceExtension ;
    rdfs:range surface-model:Content .

surface-model:hasFormat a owl:ObjectProperty ;
    rdfs:label "Object property: hasFormat"@en ;
    rdfs:comment "Links a DataResourceExtension to an instance of surface-model:Format that describes the surface model's file format details."@en ;
    rdfs:subPropertyOf envited-x:hasFormat ;
    rdfs:domain surface-model:DataResourceExtension ;
    rdfs:range surface-model:Format .
